theories/sts.v
@@ -70,60 +70,60 @@ Proof.
   solve_inG.
 Qed.
 
-(* Definition tframeR := excl_authR (leibnizO nat). *)
-(* Definition tframeUR := excl_authUR (leibnizO nat). *)
+Definition tframeR := excl_authR (leibnizO nat).
+Definition tframeUR := excl_authUR (leibnizO nat).
 
-(* Class TFRAME_preG Σ := *)
-(*   { tframe_preG :: inG Σ tframeUR; }. *)
+Class TFRAME_preG Σ :=
+  { tframe_preG :: inG Σ tframeUR; }.
 
-(* Class TFRAMEG Σ := *)
-(*   { tframe_inG :: inG Σ tframeUR; *)
-(*     γtframe : gname; *)
-(*   }. *)
+Class TFRAMEG Σ :=
+  { tframe_inG :: inG Σ tframeUR;
+    γtframe : gname;
+  }.
 
-(* Definition TFRAME_preΣ := *)
-(*   #[ GFunctor tframeUR ]. *)
+Definition TFRAME_preΣ :=
+  #[ GFunctor tframeUR ].
 
-(* Instance subG_TFRAME_preΣ {Σ} : *)
-(*   subG TFRAME_preΣ Σ → TFRAME_preG Σ. *)
-(* Proof. solve_inG. Qed. *)
+Instance subG_TFRAME_preΣ {Σ} :
+  subG TFRAME_preΣ Σ → TFRAME_preG Σ.
+Proof. solve_inG. Qed.
 
-(* Section TStack. *)
-(*   Context {Σ : gFunctors} {tframeg : TFRAMEG Σ} . *)
+Section TStack.
+  Context {Σ : gFunctors} {tframeg : TFRAMEG Σ} .
 
-(*   Definition tframe_full (a : nat) : iProp Σ *)
-(*     := own γtframe (●E a : tframeUR). *)
+  Definition tframe_full (a : nat) : iProp Σ
+    := own γtframe (●E a : tframeUR).
 
-(*   Definition tframe_frag (a : nat) : iProp Σ *)
-(*     := own γtframe (◯E a : tframeUR). *)
+  Definition tframe_frag (a : nat) : iProp Σ
+    := own γtframe (◯E a : tframeUR).
 
-(*   Lemma tframe_agree (a a' : nat) : *)
-(*    tframe_full a -∗ *)
-(*    tframe_frag a' -∗ *)
-(*    ⌜ a = a' ⌝. *)
-(*   Proof. *)
-(*     iIntros "Hfull Hfrag". *)
-(*     rewrite /tframe_full /tframe_frag. *)
-(*     iCombine "Hfull Hfrag" as "H". *)
-(*     iDestruct (own_valid with "H") as "%H". *)
-(*     by apply excl_auth_agree_L in H. *)
-(*   Qed. *)
+  Lemma tframe_agree (a a' : nat) :
+   tframe_full a -∗
+   tframe_frag a' -∗
+   ⌜ a = a' ⌝.
+  Proof.
+    iIntros "Hfull Hfrag".
+    rewrite /tframe_full /tframe_frag.
+    iCombine "Hfull Hfrag" as "H".
+    iDestruct (own_valid with "H") as "%H".
+    by apply excl_auth_agree_L in H.
+  Qed.
 
-(*   Lemma tframe_update (a a' a'' : nat) : *)
-(*    tframe_full a -∗ *)
-(*    tframe_frag a' ==∗ *)
-(*    tframe_full a'' ∗ tframe_frag a''. *)
-(*   Proof. *)
-(*     iIntros "Hfull Hfrag". *)
-(*     rewrite /tframe_full /tframe_frag. *)
-(*     iCombine "Hfull Hfrag" as "H". *)
-(*     iMod ( own_update _ _ _  with "H" ) as "H". *)
-(*     { apply excl_auth_update. } *)
-(*     iDestruct "H" as "[? ?]". *)
-(*     by iFrame. *)
-(*   Qed. *)
+  Lemma tframe_update (a a' a'' : nat) :
+   tframe_full a -∗
+   tframe_frag a' ==∗
+   tframe_full a'' ∗ tframe_frag a''.
+  Proof.
+    iIntros "Hfull Hfrag".
+    rewrite /tframe_full /tframe_frag.
+    iCombine "Hfull Hfrag" as "H".
+    iMod ( own_update _ _ _  with "H" ) as "H".
+    { apply excl_auth_update. }
+    iDestruct "H" as "[? ?]".
+    by iFrame.
+  Qed.
 
-(* End TStack. *)
+End TStack.
 
 Section definitionsS.
 
@@ -246,19 +246,19 @@ Proof.
   apply encode_inj in HH2. subst; eauto.
 Qed.
 
-(* Section pre_TFRAME. *)
-(*   Context {Σ : gFunctors} {tframeg : TFRAME_preG Σ}. *)
+Section pre_TFRAME.
+  Context {Σ : gFunctors} {tframeg : TFRAME_preG Σ}.
 
-(*   Lemma gen_tframe_init (n : nat) : *)
-(*     ⊢ |==> (∃ (tframeg : TFRAMEG Σ), tframe_full n ∗ tframe_frag n). *)
-(*   Proof. *)
-(*     iMod (own_alloc (A:=tframeUR) (●E n ⋅ ◯E n )) as (γtframe) "Htframe" *)
-(*     ; first by apply excl_auth_valid. *)
-(*     iModIntro. iExists (Build_TFRAMEG _ _ γtframe). *)
-(*     by rewrite own_op. *)
-(*   Qed. *)
+  Lemma gen_tframe_init (n : nat) :
+    ⊢ |==> (∃ (tframeg : TFRAMEG Σ), tframe_full n ∗ tframe_frag n).
+  Proof.
+    iMod (own_alloc (A:=tframeUR) (●E n ⋅ ◯E n )) as (γtframe) "Htframe"
+    ; first by apply excl_auth_valid.
+    iModIntro. iExists (Build_TFRAMEG _ _ γtframe).
+    by rewrite own_op.
+  Qed.
 
-(* End pre_TFRAME. *)
+End pre_TFRAME.
 
 Section pre_STS.
   Context {A B E D: Type} {Σ : gFunctors} {eqa: EqDecision A} {compare_a: Ord A}
